feat: execute relation for SQS

spec/SQS.thy
@@ -23,6 +23,9 @@ datatype 'a SQSRequestPayload
 
 datatype 'a SQSRequest = SQSRequest ClientId "'a SQSRequestPayload"
 
+fun getRequestPayload where
+  "getRequestPayload (SQSRequest _ p) = p"
+
 datatype 'a SQSResponsePayload
   = Returned "(MessageId \<times> 'a) list"
 
@@ -40,6 +43,33 @@ fun steps :: "('s \<Rightarrow> 'q \<Rightarrow> 's \<times> 'p option) \<Righta
   "steps f s0 [] = (s0, [])"
 | "steps f s (q#qs) = (let (s',p') = f s q in let (s'',ps) = steps f s' qs in (s'', case p' of None \<Rightarrow> ps | Some(p) \<Rightarrow> p # ps))"
 
+lemma steps_cons_destruct[elim]:
+  fixes s :: "'a SQSState"
+  assumes "steps f s (q#qs) = (s',ps)"
+  obtains s'' p' ps' where "(s'',p') = f s q" "(s',ps') = steps f s'' qs" "ps = (case p' of None \<Rightarrow> ps' | Some(p) \<Rightarrow> p # ps')"
+  using assms
+  apply (cases "f s q")
+  apply simp
+proof-
+  fix a :: "'a SQSState" and b
+  assume hyp: "(\<And>s'' p' ps'. s'' = a \<and> p' = b \<Longrightarrow> (s', ps') = steps f a qs \<Longrightarrow> ps = (case b of None \<Rightarrow> ps' | Some p \<Rightarrow> p # ps') \<Longrightarrow> thesis)"
+    and t: "(case steps f a qs of (s'', ps) \<Rightarrow> (s'', case b of None \<Rightarrow> ps | Some p \<Rightarrow> p # ps)) = (s', ps)"
+    and s: "f s q = (a, b)"
+
+  have "fst (steps f a qs) = s'"
+    by (metis (no_types, lifting) case_prod_beta fst_conv t)
+  have "ps = (case b of None \<Rightarrow> snd (steps f a qs) | Some p \<Rightarrow> p # snd (steps f a qs))"
+    using t
+    apply (cases "steps f a qs")
+    using sndI by fastforce
+
+  show thesis
+    apply (rule hyp [of a b "snd (steps f a qs)"])
+    apply simp
+    using \<open>fst (steps f a qs) = s'\<close> apply auto[1]
+    by (simp add: \<open>ps = (case b of None \<Rightarrow> snd (steps f a qs) | Some p \<Rightarrow> p # snd (steps f a qs))\<close>)
+qed
+
 lemma "steps SQS_step initialSQSState [] = (initialSQSState, [])"
   by simp
 
@@ -52,5 +82,62 @@ lemma "steps SQS_step (initialSQSState :: nat SQSState) [
   (\<lparr> messages = [(MessageId 1, 5), (MessageId 2, 1)], messageIdCounter = 3 \<rparr> :: nat SQSState,
   [SQSResponse (ClientId 0) (Returned [(MessageId 0, 10), (MessageId 1, 5), (MessageId 2, 1)])])"
   by (simp add: initialSQSState_def)
+
+inductive SQS_execute where
+  SQS_execute_empty: "SQS_execute st [] st []"
+| SQS_execute_step: "\<lbrakk> SQS_step st q = (st', p); SQS_execute st' qs st'' ps \<rbrakk> \<Longrightarrow> SQS_execute st (q#qs) st'' (case p of None \<Rightarrow> ps | Some(p) \<Rightarrow> p # ps)"
+
+lemma SQS_steps_to_execute:
+  fixes st :: "'a SQSState"
+  shows "(st',ps) = steps SQS_step st qs \<Longrightarrow> SQS_execute st qs st' ps"
+  apply (induct qs arbitrary: st st' ps)
+  apply (simp, rule)
+proof-
+  fix a qs and st :: "'a SQSState" and st' ps
+  assume "(\<And>st st' ps. (st', ps) = steps SQS_step st qs \<Longrightarrow> SQS_execute st qs st' ps)"
+    and "(st', ps) = steps SQS_step st (a # qs)"
+  obtain s'' p' ps' where q: "(s'',p') = SQS_step st a" "(st',ps') = steps SQS_step s'' qs" "ps = (case p' of None \<Rightarrow> ps' | Some(p) \<Rightarrow> p # ps')"
+    by (metis \<open>(st', ps) = steps SQS_step st (a # qs)\<close> steps_cons_destruct)
+
+  show "SQS_execute st (a # qs) st' ps"
+    apply (simp add: q(3))
+    apply rule
+    apply (simp add: q(1) [symmetric])
+    by (simp add: \<open>\<And>st' st ps. (st', ps) = steps SQS_step st qs \<Longrightarrow> SQS_execute st qs st' ps\<close> q(2))
+qed
+
+lemma SQS_execute_to_steps:
+  fixes st :: "'a SQSState"
+  shows "SQS_execute st qs st' ps \<Longrightarrow> steps SQS_step st qs = (st',ps)"
+  apply (induct rule: SQS_execute.induct)
+  apply simp
+  apply simp
+  done
+
+theorem SQS_execute_iff_steps:
+  fixes st :: "'a SQSState"
+  shows "SQS_execute st qs st' ps = (steps SQS_step st qs = (st',ps))"
+  using SQS_execute_to_steps SQS_steps_to_execute by force
+
+lemma
+  assumes "SQS_execute st [m] st' ps" and "getRequestPayload m = Send v"
+  obtains mid where "messages st' = messages st @ [(mid, v)]" "mid = MessageId (messageIdCounter st)"
+proof-
+  have "steps SQS_step st [m] = (st',ps)"
+    using assms
+    using SQS_execute_to_steps by blast
+  hence "messages st' = messages st @ [(MessageId (messageIdCounter st), v)]"
+    apply (simp)
+    apply (cases "SQS_step st m")
+    apply simp
+    using assms(2)
+    apply (cases m)
+    apply auto
+    done
+
+  assume "(\<And>mid. messages st' = messages st @ [(mid, v)] \<Longrightarrow> mid = MessageId (messageIdCounter st) \<Longrightarrow> thesis)"
+  show thesis
+    using \<open>messages st' = messages st @ [(MessageId (messageIdCounter st), v)]\<close> that by blast
+qed
 
 end
